format-version: 1.2
date: 13:08:2012 11:25
saved-by: midori
default-namespace: fypo_extensions
ontology: fypo_extensions
remark: collection (perhaps temporary) of terms allowed in FYPO annotation has_penetrance and has_expressivity extensions

[Term]
id: FYPO_EXT:0000001
name: high
def: "large fraction of cells (penetrance) or strong phenotype (expressivity)" [PomBase:curators]
is_a: FYPO_EXT:1000000 ! FYPO extension

[Term]
id: FYPO_EXT:0000002
name: medium
def: "intermediate fraction of cells (penetrance) or moderate phenotype (expressivity)" [PomBase:curators]
is_a: FYPO_EXT:1000000 ! FYPO extension

[Term]
id: FYPO_EXT:0000003
name: low
def: "small fraction of cells (penetrance) or weak phenotype (expressivity)" [PomBase:curators]
is_a: FYPO_EXT:1000000 ! FYPO extension

[Term]
id: FYPO_EXT:0000004
name: complete
def: "all cells (penetrance)" [PomBase:curators]
synonym: "100%" EXACT PomBase:curators]
synonym: "full" EXACT PomBase:curators]
is_a: FYPO_EXT:0000001 ! high

[Term]
id: FYPO_EXT:1000000
name: FYPO extension
def: "root of FYPO extension ontology" [PomBase:mah]
